HOL_To_IMP/HOL_Nat_To_IMP/Automation/HOL_Nat_To_IMP_Goal_Commands.thy
@@ -1,0 +1,11 @@
+\<^marker>\<open>creator "Kevin Kappelmann"\<close>
+theory HOL_Nat_To_IMP_Goal_Commands
+  imports
+    HOL_Nat_To_IMP_Utils
+    Compile_HOL_Nat_To_IMP
+  keywords "HOL_To_IMP_correct" :: thy_goal_defn
+begin
+
+ML_file\<open>hol_nat_to_imp_goal_command.ML\<close>
+
+end
