HOL_To_IMP/HOL_Nat_To_IMP/HOL_Nat_To_IMP_Base.thy
@@ -1,5 +1,5 @@
 \<^marker>\<open>creator "Kevin Kappelmann"\<close>
-theory HOL_Nat_To_IMP_Minus_Base
+theory HOL_Nat_To_IMP_Base
   imports
     HOL.HOL
     ML_Unification.ML_Tactic_Utils
@@ -15,13 +15,13 @@ locale HOL_To_HOL_Nat
 begin
 end
 
-locale HOL_Nat_To_IMP_Minus
+locale HOL_Nat_To_IMP
 begin
 sublocale HTHN : HOL_To_HOL_Nat .
 end
 
-setup_result HOL_Nat_To_IMP_Minus_base_logger =
-  \<open>Logger.new_logger Logger.root "HOL_Nat_To_IMP_Minus_Base"\<close>
+setup_result HOL_Nat_To_IMP_base_logger =
+  \<open>Logger.new_logger Logger.root "HOL_Nat_To_IMP_Base"\<close>
 
 ML_file\<open>hol_nat_to_imp_util.ML\<close>
 
