HOL_To_IMP/Refinements/HOL_To_IMP_Arithmetics.thy
@@ -1,7 +1,7 @@
 \<^marker>\<open>creator "Kevin Kappelmann"\<close>
-theory HOL_To_IMP_Minus_Arithmetics
+theory HOL_To_IMP_Arithmetics
   imports
-    HOL_To_IMP_Minus_Primitives
+    HOL_To_IMP_Primitives
     "HOL-Library.Discrete_Functions"
 begin
 
@@ -29,15 +29,15 @@ function_compile_nat power_eq_power_acc_nat_one
 
 end
 
-context HOL_Nat_To_IMP_Minus
+context HOL_Nat_To_IMP
 begin
 
 lemmas power_acc_nat_nat_eq = HTHN.power_acc_nat_nat_eq_unfolded[unfolded case_nat_eq_if]
 compile_nat power_acc_nat_nat_eq basename power_acc
-HOL_To_IMP_Minus_correct HTHN.power_acc_nat_nat by cook
+HOL_To_IMP_correct HTHN.power_acc_nat_nat by cook
 
 compile_nat HTHN.power_nat_eq_unfolded basename power
-HOL_To_IMP_Minus_correct HTHN.power_nat by cook
+HOL_To_IMP_correct HTHN.power_nat by cook
 
 end
 
@@ -94,23 +94,23 @@ function_compile_nat sqrt_nat_def
 
 end
 
-context HOL_Nat_To_IMP_Minus
+context HOL_Nat_To_IMP
 begin
 
 compile_nat HTHN.sqrt_aux_nat_nat_eq_unfolded
-HOL_To_IMP_Minus_correct HTHN.sqrt_aux_nat_nat by cook
+HOL_To_IMP_correct HTHN.sqrt_aux_nat_nat by cook
   (*Example step-by-step tactic invocation for debugging purposes.*)
   (* apply (tactic \<open>HM.correct_if_IMP_tailcall_correct_tac HT.get_IMP_def @{context} 1\<close>)
   apply (tactic \<open>HT.setup_induction_tac HT.get_fun_inducts @{context} 1\<close>)
   apply (tactic \<open>HT.start_case_tac HT.get_IMP_def @{context} 1\<close>)
-  apply (tactic \<open>HT.run_tac HT.get_imp_minus_correct @{context} 1\<close>)
+  apply (tactic \<open>HT.run_tac HT.get_imp_correct @{context} 1\<close>)
   apply (tactic \<open>SOLVED' (HT.finish_tac HB.get_HOL_eqs @{context}) 1\<close>)
   apply (tactic \<open>SOLVED' (HT.finish_tac HB.get_HOL_eqs @{context}) 1\<close>)
   apply (tactic \<open>SOLVED' (HT.finish_tac HB.get_HOL_eqs @{context}) 1\<close>)
   oops *)
 
 compile_nat HTHN.sqrt_nat_nat_eq_unfolded
-HOL_To_IMP_Minus_correct HTHN.sqrt_nat_nat by cook
+HOL_To_IMP_correct HTHN.sqrt_nat_nat by cook
 
 end
 
