HOL_To_IMP/Refinements/HOL_To_IMP_IS_To_VC.thy
@@ -1,7 +1,7 @@
 \<^marker>\<open>creator "Nico Lintner"\<close>
-theory HOL_To_IMP_Minus_IS_To_VC
+theory HOL_To_IMP_IS_To_VC
   imports
-    HOL_To_IMP_Minus_Lists
+    HOL_To_IMP_Lists
     Karp21.IS_To_VC_List
 begin
 
@@ -13,12 +13,12 @@ function_compile_nat list_card_eq
 
 end
 
-context HOL_Nat_To_IMP_Minus
+context HOL_Nat_To_IMP
 begin
 
 lemmas list_card_nat_eq = HTHN.list_card_nat_eq_unfolded
 compile_nat list_card_nat_eq
-HOL_To_IMP_Minus_correct HOL_To_HOL_Nat.list_card_nat by cook
+HOL_To_IMP_correct HOL_To_HOL_Nat.list_card_nat by cook
 
 end
 
@@ -29,22 +29,22 @@ function_compile_nat is_vc_list_def
 
 end
 
-context HOL_Nat_To_IMP_Minus
+context HOL_Nat_To_IMP
 begin
 
 lemmas is_vc_list_nat_eq = HTHN.is_vc_list_nat_eq_unfolded[unfolded case_prod_nat_def]
 compile_nat is_vc_list_nat_eq
-HOL_To_IMP_Minus_correct HOL_To_HOL_Nat.is_vc_list_nat by (cook mode = induction)
+HOL_To_IMP_correct HOL_To_HOL_Nat.is_vc_list_nat by (cook mode = induction)
 
-lemma is_vc_list_IMP_Minus_correct:
+lemma is_vc_list_IMP_correct:
   assumes "Rel_nat (s ''is_vc_list_nat.arg.x'') x"
-  shows "terminates_with_res_IMP_Minus (tailcall_to_IMP_Minus is_vc_list_nat_IMP_tailcall) s
+  shows "terminates_with_res_IMP (tailcall_to_IMP is_vc_list_nat_IMP_tailcall) s
     ''is_vc_list_nat.ret'' (natify (is_vc_list x))"
 proof -
   have "HTHN.is_vc_list_nat TYPE('a) (s ''is_vc_list_nat.arg.x'') = natify (is_vc_list x)"
     using HTHN.is_vc_list_nat_eq_unfolded[OF assms] HTHN.Rel_nat_is_vc_list_nat_unfolded[OF assms]
     by (simp add: Rel_nat_iff_eq_natify)
-  then show ?thesis using is_vc_list_nat_IMP_Minus_correct[of s, OF assms] by simp
+  then show ?thesis using is_vc_list_nat_IMP_correct[of s, OF assms] by simp
 qed
 
 end
