HOL_To_IMP/Refinements/HOL_To_IMP_Pairs.thy
@@ -1,7 +1,7 @@
 \<^marker>\<open>creator "Kevin Kappelmann"\<close>
-theory HOL_To_IMP_Minus_Pairs
+theory HOL_To_IMP_Pairs
   imports
-    HOL_To_IMP_Minus_Arithmetics
+    HOL_To_IMP_Arithmetics
 begin
 
 context HOL_To_HOL_Nat
@@ -16,24 +16,24 @@ function_compile_nat rpair_def
 
 end
 
-context HOL_Nat_To_IMP_Minus
+context HOL_Nat_To_IMP
 begin
 
 declare Rel_nat_selector_prod[Rel_nat]
 
 compile_nat Pair_nat_def
-HOL_To_IMP_Minus_correct Pair_nat by cook
+HOL_To_IMP_correct Pair_nat by cook
 
 lemmas fst_nat_eq = HTHN.fst_nat_eq_unfolded[unfolded case_prod_nat_def]
 compile_nat fst_nat_eq
-HOL_To_IMP_Minus_correct HOL_To_HOL_Nat.fst_nat by cook
+HOL_To_IMP_correct HOL_To_HOL_Nat.fst_nat by cook
 
 lemmas snd_nat_eq = HTHN.snd_nat_eq_unfolded[unfolded case_prod_nat_def]
 compile_nat snd_nat_eq
-HOL_To_IMP_Minus_correct HOL_To_HOL_Nat.snd_nat by cook
+HOL_To_IMP_correct HOL_To_HOL_Nat.snd_nat by cook
 
 compile_nat HTHN.rpair_nat_eq_unfolded
-HOL_To_IMP_Minus_correct HOL_To_HOL_Nat.rpair_nat by cook
+HOL_To_IMP_correct HOL_To_HOL_Nat.rpair_nat by cook
 
 end
 
