HOL_To_IMP/Refinements/HOL_To_IMP_SAT.thy
@@ -1,8 +1,8 @@
 \<^marker>\<open>creator "Kevin Kappelmann"\<close>
 \<^marker>\<open>creator "Nico Lintner"\<close>
-theory HOL_To_IMP_Minus_SAT
+theory HOL_To_IMP_SAT
   imports
-    HOL_To_IMP_Minus_Lists
+    HOL_To_IMP_Lists
     Karp21.SAT_List_Definition
 begin
 
@@ -26,32 +26,30 @@ case_of_simps map_lit_eq : lit.map
 
 end
 
-context HOL_Nat_To_IMP_Minus
+context HOL_Nat_To_IMP
 begin
 
 declare Rel_nat_selector_lit[Rel_nat]
 
 compile_nat Pos_nat_def
-HOL_To_IMP_Minus_correct Pos_nat by cook
+HOL_To_IMP_correct Pos_nat by cook
 
 compile_nat Neg_nat_def
-HOL_To_IMP_Minus_correct Neg_nat by cook
+HOL_To_IMP_correct Neg_nat by cook
 
 compile_nat HTHN.is_n_clause_list_nat_eq_unfolded
-HOL_To_IMP_Minus_correct HOL_To_HOL_Nat.is_n_clause_list_nat by cook
+HOL_To_IMP_correct HOL_To_HOL_Nat.is_n_clause_list_nat by cook
 
 lemmas is_n_sat_list_nat_eq = HTHN.is_n_sat_list_nat_eq_unfolded[unfolded
   case_list_nat_def case_bool_nat_def]
 compile_nat is_n_sat_list_nat_eq
-HOL_To_IMP_Minus_correct HOL_To_HOL_Nat.is_n_sat_list_nat
+HOL_To_IMP_correct HOL_To_HOL_Nat.is_n_sat_list_nat
   apply (tactic \<open>HM.correct_if_IMP_tailcall_correct_tac HT.get_IMP_def @{context} 1\<close>)
-  by (induction ya arbitrary: s)
-  (tactic \<open>PARALLEL_ALLGOALS (HT.start_run_finish_case_tac HT.get_IMP_def HT.get_imp_minus_correct
-    HB.get_HOL_eqs @{context})\<close>)
+  by (induction ya arbitrary: s) (cook mode = run_finish)
 
 lemmas flip_lit_nat_eq = HTHN.flip_lit_nat_eq_unfolded[unfolded case_lit_nat_def]
 compile_nat flip_lit_nat_eq
-HOL_To_IMP_Minus_correct HOL_To_HOL_Nat.flip_lit_nat by cook
+HOL_To_IMP_correct HOL_To_HOL_Nat.flip_lit_nat by cook
 
 end
 
