Paper/Syntax.thy
@@ -1,6 +1,6 @@
 theory Syntax
   imports "IMP_To_IMP-.IMP_To_IMP_Minus" "IMP.IMP_Tailcall" "IMP-.IMP_Minus_Big_StepT"
-    "HOL_Nat_To_IMP-.IMP_Terminates_With"
+    "HOL_Nat_To_IMP.IMP_Terminates_With"
 begin
 
 (* disabled: original syntax *)
@@ -15,7 +15,7 @@ no_notation tail_steps ("_ \<turnstile>''_ \<Rightarrow>\<^bsup>_\<^esup>  _" 55
 (* terminates with syntax *)
 bundle terminates_with_syntax
 begin
-  notation terminates_with_res_IMP_Minus ("'(_, _') \<Rightarrow>\<^bsub>_\<^esub> _")
+  notation terminates_with_res_IMP ("'(_, _') \<Rightarrow>\<^bsub>_\<^esub> _")
   notation terminates_with_res_IMP_Tailcall ("_ \<turnstile> '(_, _') \<Rightarrow>\<^bsub>_\<^esub> _")
   notation terminates_with_IMP_Tailcall ("_ \<turnstile> '(_, _') \<Rightarrow> _")
 end
